theories/Effect.v
@@ -1,0 +1,268 @@
+(* This Source Code Form is subject to the terms of the Mozilla Public
+ * License, v. 2.0. If a copy of the MPL was not distributed with this
+ * file, You can obtain one at https://mozilla.org/MPL/2.0/. *)
+
+(* Copyright (C) 2018–2020 ANSSI *)
+
+From FreerDPS Require Import Init.
+
+(** * Definition  *)
+
+(** Following the definition of the <<operational>> package, effects in
+    FreeSpec are parameterized inductive types whose terms purposely describe
+    the primitives the effect provides. *)
+
+Definition effect := Type -> Type.
+
+Declare Scope effect_scope.
+Bind Scope effect_scope with effect.
+
+(** Given [F : effect], a term of type [F α] identifies a primitive of [F]
+    expected to produce a result of type [α].
+
+    The simpler effect is the empty effect, which provides no primitives
+    whatsoever. *)
+
+Inductive eempty : effect := .
+
+(** Another example of general-purpose effect we can define is the [STORE s]
+    effect, where [s] is a type for a state, and [STORE s] allows for
+    manipulating a global, mutable variable of type [s] within an impure
+    computation. *)
+
+Inductive STORE (s : Type) : effect :=
+| Get : STORE s s
+| Put (x : s) : STORE s unit.
+
+Arguments Get {s}.
+Arguments Put [s] (x).
+
+(** According to the definition of [STORE s], an impure computation can use two
+    primitives. The term [Get : STORE s s] describes a primitive expected to
+    produce a result of type [s], that is the current value of the mutable
+    variable.  Terms of the form [Put x : STORE s unit] describe a primitive
+    which does not produce any meaningful result, but is expected to update the
+    current value of the mutable variable.
+
+    The use of the word “expected” to describe the primitive of [STORE s] is
+    voluntary.  The definition of an effect does not attach any particular
+    semantics to the primitives it describes.  This will come later, and in
+    fact, one effect may have many legitimate semantics.
+
+    Impure computations are likely to use more than one effect, but the
+    [impure] monad takes only one argument.  We introduce [eplus] (denoted by
+    [<+>] or [⊕]) to compose effects together.  An impure computation
+    parameterized by [F ⊕ E] can therefore leverage the primitives of both [F]
+    and [E]. *)
+
+(** * Polymorphic Effect Composites *)
+
+(** When defining general-purpose impure computations that we expect to reuse in
+    different context, we want to leave the effect as a parameter, and rather
+    express the constraints in terms of effect availability.  We tackle this
+    challenge by means of _effect composites_.
+
+    - We say an effect composite [ix] _provides_ a concrete effect [i]
+      when there exists a function [inj_p : forall α, i α -> ix α].
+    - Conversely, we can determine if a primitive of an effect composite [ix]
+      is forwarded to a concrete effect [i] when there exists a function
+      [proj_p : forall α, ix α -> option (i a)].
+
+    We encode this mechanics using two type classes: [MayProvide], and
+    [Provide]. *)
+
+Class MayProvide (ix i : effect) : Type :=
+  { proj_p {α} (e : ix α) : option (i α)
+  }.
+
+Class Provide (ix i : effect) `{MayProvide ix i} : Type :=
+  { inj_p {α} (e : i α) : ix α
+  ; proj_inj_p_equ {α} (e : i α) : proj_p (inj_p e) = Some e
+  }.
+
+(** We provide a default instance for [MayProvide] in the form of a function
+    [proj_p] which always return [None].  We give to this default instance a
+    ridiculously high priority number to ensure it is selected only if no other
+    instances are found. *)
+
+Instance default_MayProvide (i j : effect) : MayProvide i j|1000 :=
+  { proj_p := fun _ _ => None
+  }.
+
+(** It is expected that, for an effect composite [ix] which provides [i] and
+    may provide [j], [inj_p] and [proj_p] do not mix up [i] and [j]
+    primitives. That is, injecting a primitive [e] of [i] inside [ix], then
+    projecting the resulting primitive into [j] returns [None] as long as [i]
+    and [j] are two different effects. *)
+
+Class Distinguish (ix i j : effect) `{Provide ix i, MayProvide ix j} : Prop :=
+  { distinguish : forall {α} (e : i α), proj_p (i := j) (inj_p (ix := ix) e) = None
+  }.
+
+(** * Composing Effects *)
+
+(** We provide the [eplus] operator to compose effects together. That is,
+    [eplus] can be used to build _concrete_ (as opposed to polymorphic)
+    effect composite. *)
+
+Inductive eplus (i j : effect) (α : Type) :=
+| in_left (e : i α) : eplus i j α
+| in_right (e : j α) : eplus i j α.
+
+Arguments in_left [i j α] (e).
+Arguments in_right [i j α] (e).
+
+Register eplus as freespec.core.eplus.type.
+Register in_left as freespec.core.eplus.in_left.
+Register in_right as freespec.core.eplus.in_right.
+
+Infix "+" := eplus : effect_scope.
+
+(** For [eplus] to be used seamlessly as a concrete effect composite, we
+    provide the necessary instances for the [MayProvide], [Provide] and
+    [Distinguish] type classes. Note that these instances always prefer the
+    left operand of [eplus]. For instance, considering a situation where
+    there is an instance for [Provide ix i] and an instance for [Provide jx i],
+    the instance of [Provide (ix + jx) i] will rely on [ix].
+
+    The main use case for [eplus] is to locally provide an additional
+    effect. For instance, we can consider a [with_state] function which would
+    locally give access to the [STORE] effect, that is [with_state : forall
+    ix s α, s -> impure (ix + STORE s) α -> impure ix α]. In such a case, the
+    effect made locally available shall be the right operand of [eplus]. This
+    way, functions such as [with_state] are reentrant. If we take an example,
+    the following impure computation:
+
+<<
+with_state true (with_state false get)
+>>
+
+    will return false (that is, the variable in the inner store). *)
+
+Instance refl_MayProvide (i : effect) : MayProvide i i :=
+  { proj_p := fun _ e => Some e
+  }.
+
+#[program]
+Instance refl_Provide (i : effect) : @Provide i i (refl_MayProvide i) :=
+  { inj_p := fun (a : Type) (e : i a) => e
+  }.
+
+Instance eplus_left_MayProvide (ix i j : effect) `{MayProvide ix i}
+  : MayProvide (ix + j) i :=
+  { proj_p := fun _ e =>
+                match e with
+                | in_left e => proj_p e
+                | _ => None
+                end
+  }.
+
+#[program]
+Instance eplus_left_Provide (ix i j : effect) `{Provide ix i}
+  : @Provide (ix + j) i (eplus_left_MayProvide ix i j) :=
+  { inj_p := fun (a : Type) (e : i a) => in_left (inj_p e)
+  }.
+
+Next Obligation.
+  now rewrite proj_inj_p_equ.
+Qed.
+
+Instance eplus_right_MayProvide (i jx j : effect) `{MayProvide jx j}
+  : MayProvide (i + jx) j :=
+  { proj_p := fun _ e =>
+                match e with
+                | in_right e => proj_p e
+                | _ => None
+                end
+  }.
+
+#[program]
+Instance eplus_right_Provide (i jx j : effect) `{Provide jx j}
+  : @Provide (i + jx) j (eplus_right_MayProvide i jx j) :=
+  { inj_p := fun _ e => in_right (inj_p e)
+  }.
+
+Next Obligation.
+  now rewrite proj_inj_p_equ.
+Qed.
+
+(** By default, Coq's inference algorithm for type classe instances inference is
+    a depth-first search. This is not without consequence in our case. For
+    instance, if we consider the search of an instance for [MayProvide (i + j)
+    j], Coq will first try [eplus_right_MayProvide] (as explained previously),
+    meaning he now search for [MayProvide i j]. It turns out such an instance
+    exists: [default_MayProvide].
+
+    To circumvent this issue, we write a dedicated tactic [find_may_provide]
+    which attempts to find an instance for [MayProvide (?ix + ?jx) ?i] with
+    [refl_MayProvide], [eplus_left_MayProvide] and [eplus_right_MayProvide]. *)
+
+Ltac find_may_provide :=
+  eapply refl_MayProvide +
+  (eapply eplus_left_MayProvide; find_may_provide) +
+  (eapply eplus_right_MayProvide; find_may_provide).
+
+#[global] Hint Extern 1 (MayProvide (eplus _ _) _) =>
+  find_may_provide : typeclass_instances.
+
+#[program]
+Instance refl_Distinguish (i j : effect)
+  : @Distinguish i i j  ( @refl_MayProvide i) ( @refl_Provide i) ( @default_MayProvide i j).
+
+#[program]
+Instance eplus_left_default_Distinguish (ix jx i j : effect)
+   `{M1 : MayProvide ix i} `{P1 : @Provide ix i M1}
+  : @Distinguish (ix + jx) i j
+                 ( @eplus_left_MayProvide ix i jx M1)
+                 ( @eplus_left_Provide ix i jx M1 P1)
+                 ( @default_MayProvide _ j).
+
+#[program]
+Instance eplus_right_default_Distinguish (ix jx i j : effect)
+   `{M1 : MayProvide jx i} `{P1 : @Provide jx i M1}
+  : @Distinguish (ix + jx) i j
+                 ( @eplus_right_MayProvide ix jx i M1)
+                 ( @eplus_right_Provide ix jx i M1 P1)
+                 ( @default_MayProvide _ j).
+
+#[program]
+Instance eplus_left_may_right_Distinguish (ix jx i j : effect)
+   `{M1 : MayProvide ix i} `{P1 : @Provide ix i M1} `{M2 : MayProvide jx j}
+  : @Distinguish (ix + jx) i j
+                 ( @eplus_left_MayProvide ix i jx M1)
+                 ( @eplus_left_Provide ix i jx M1 P1)
+                 ( @eplus_right_MayProvide ix jx j M2).
+
+#[program]
+Instance eplus_right_may_left_Distinguish (ix jx i j : effect)
+   `{M1 : MayProvide jx i} `{P1 : @Provide jx i M1} `{M2 : MayProvide ix j}
+  : @Distinguish (ix + jx) i j
+                 ( @eplus_right_MayProvide ix jx i M1)
+                 ( @eplus_right_Provide ix jx i M1 P1)
+                 ( @eplus_left_MayProvide ix j jx M2).
+
+#[program]
+Instance eplus_left_distinguish_left_Distinguish (ix jx i j : effect)
+   `{M1 : MayProvide ix i} `{P1 : @Provide ix i M1} `{M2 : MayProvide ix j}
+   `{@Distinguish ix i j M1 P1 M2}
+  : @Distinguish (ix + jx) i j
+                 ( @eplus_left_MayProvide ix i jx M1)
+                 ( @eplus_left_Provide ix i jx M1 P1)
+                 ( @eplus_left_MayProvide ix j jx M2).
+
+Next Obligation.
+  apply distinguish.
+Defined.
+
+#[program]
+Instance eplus_right_distinguish_right_Distinguish (ix jx i j : effect)
+   `{M1 : MayProvide jx i} `{P1 : @Provide jx i M1} `{M2 : MayProvide jx j}
+   `{@Distinguish jx i j M1 P1 M2}
+  : @Distinguish (ix + jx) i j
+                 ( @eplus_right_MayProvide ix jx i M1)
+                 ( @eplus_right_Provide ix jx i M1 P1)
+                 ( @eplus_right_MayProvide ix jx j M2).
+
+Next Obligation.
+  apply distinguish.
+Defined.
